books/str/strline.lisp
@@ -1,0 +1,214 @@
+; ACL2 String Library
+; Copyright (C) 2009-2010 Centaur Technology
+;
+; Contact:
+;   Centaur Technology Formal Verification Group
+;   7600-C N. Capital of Texas Highway, Suite 300, Austin, TX 78731, USA.
+;   http://www.centtech.com/
+;
+; This program is free software; you can redistribute it and/or modify it under
+; the terms of the GNU General Public License as published by the Free Software
+; Foundation; either version 2 of the License, or (at your option) any later
+; version.  This program is distributed in the hope that it will be useful but
+; WITHOUT ANY WARRANTY; without even the implied warranty of MERCHANTABILITY or
+; FITNESS FOR A PARTICULAR PURPOSE.  See the GNU General Public License for
+; more details.  You should have received a copy of the GNU General Public
+; License along with this program; if not, write to the Free Software
+; Foundation, Inc., 51 Franklin Street, Suite 500, Boston, MA 02110-1335, USA.
+;
+; Original author: Jared Davis <jared@centtech.com>
+
+(in-package "STR")
+(include-book "doc")
+(local (include-book "make-event/assert" :dir :system))
+(local (include-book "arithmetic"))
+
+(defund charpos-aux (x n xl char)
+  (declare (type string x)
+           (type integer n)
+           (type integer xl)
+           (type character char)
+           (xargs :guard (and (stringp x)
+                              (natp n)
+                              (natp xl)
+                              (<= n xl)
+                              (= xl (length x)))
+                  :measure (nfix (- (nfix xl) (nfix n)))))
+  (cond ((mbe :logic (zp (- (nfix xl) (nfix n)))
+              :exec (= n xl))
+         nil)
+        ((eql (char x n) char)
+         (mbe :logic (nfix n)
+              :exec n))
+        (t
+         (charpos-aux x
+                      (mbe :logic (+ 1 (nfix n)) :exec (+ 1 n))
+                      xl
+                      char))))
+
+(defthm charpos-aux-is-position-ac-of-nthcdr
+  (implies (and (stringp x)
+                (natp n)
+                (= xl (length x)))
+           (equal (charpos-aux x n xl char)
+                  (position-ac char (nthcdr n (coerce x 'list)) n)))
+  :hints(("Goal" :in-theory (enable charpos-aux position-ac))))
+
+(defthm position-ac-lower-bound
+  (implies (and (position-ac item x acc)
+                (natp acc))
+           (<= acc (position-ac item x acc)))
+  :rule-classes ((:rewrite) (:linear))
+  :hints(("Goal" :in-theory (enable position-ac))))
+
+(defthm position-ac-upper-bound
+  (implies (natp acc)
+           (<= (position-ac item x acc)
+               (+ acc (len x))))
+  :rule-classes ((:rewrite) (:linear))
+  :hints(("Goal" :in-theory (enable position-ac))))
+
+
+
+
+(defund go-to-line (x n xl curr goal)
+  (declare (xargs :guard (and (stringp x)
+                              (natp n)
+                              (natp xl)
+                              (<= n xl)
+                              (= xl (length x))
+                              (natp curr)
+                              (natp goal))
+                  :measure (nfix (- (nfix xl) (nfix n))))
+           (type string x)
+           (type integer n xl curr goal))
+  (cond ((mbe :logic (zp (- (nfix xl) (nfix n)))
+              :exec (= n xl))
+         nil)
+        ((= curr goal)
+         (mbe :logic (nfix n) :exec n))
+        (t
+         (go-to-line x
+                     (mbe :logic (+ 1 (nfix n)) :exec (+ 1 n))
+                     xl
+                     (if (eql (char x n) #\Newline)
+                         (+ 1 curr)
+                       curr)
+                     goal))))
+
+(defthm type-of-go-to-line
+  (or (not (go-to-line x n xl curr goal))
+      (and (integerp (go-to-line x n xl curr goal))
+           (<= 0 (go-to-line x n xl curr goal))))
+  :rule-classes :type-prescription)
+
+(defthm go-to-line-lower-bound
+  (implies (and (go-to-line x n xl curr goal)
+                (natp n))
+           (<= n (go-to-line x n xl curr goal)))
+  :rule-classes ((:rewrite) (:linear))
+  :hints(("Goal" :in-theory (enable go-to-line))))
+
+(defthm go-to-line-upper-bound
+  (implies (natp xl)
+           (<= (go-to-line x n xl curr goal)
+               xl))
+  :rule-classes ((:rewrite) (:linear))
+  :hints(("Goal" :in-theory (enable go-to-line))))
+
+
+
+(defund strline (n x)
+
+  ":Doc-Section Str
+  Extract a line from a string by its line number~/
+
+  ~c[(strline n x)] extracts the ~c[n]th line from the string ~c[x] and returns
+  it as a string.  It returns the empty string if ~c[n] does not refer to a
+  valid line.  Note that the first line is 1 (not 0).~/~/"
+
+  (declare (xargs :guard (and (posp n)
+                              (stringp x))))
+  (let* ((x     (mbe :logic (if (stringp x) x "")
+                     :exec x))
+         (xl    (length x))
+         (start (go-to-line x 0 xl 1 n)))
+    (if (not start)
+        ""
+      (let ((end (charpos-aux x start xl #\Newline)))
+        (subseq x start end)))))
+
+(defthm stringp-of-strline
+  (stringp (strline n x))
+  :rule-classes :type-prescription
+  :hints(("Goal" :in-theory (enable strline))))
+
+
+(local (acl2::assert! (equal "foo" (strline 1 "foo
+bar
+baz"))))
+
+(local (acl2::assert! (equal "bar" (strline 2 "foo
+bar
+baz"))))
+
+(local (acl2::assert! (equal "baz" (strline 3 "foo
+bar
+baz"))))
+
+(local (acl2::assert! (equal "" (strline 4 "foo
+bar
+baz"))))
+
+
+
+(defund strlines (a b x)
+  (declare (type integer a)
+           (type integer b)
+           (type string x)
+           (xargs :guard (and (posp a)
+                              (posp b)
+                              (stringp x))))
+  (let* ((x  (mbe :logic (if (stringp x) x "")
+                  :exec x))
+         (xl (length x)))
+    (mv-let
+     (a b)
+     (if (<= a b) (mv a b) (mv b a))
+     (let ((start (go-to-line x 0 xl 1 a)))
+       (if (not start)
+           ""
+         (let ((end (go-to-line x start xl a (+ 1 b))))
+           (subseq x start end)))))))
+
+(defthm stringp-of-strlines
+  (stringp (strlines a b x))
+  :rule-classes :type-prescription
+  :hints(("Goal" :in-theory (enable strlines))))
+
+
+#||
+(defconst *txt* "Line 1
+Line 2
+Line 3
+Line 4
+Line 5
+Line 6"))
+
+(strlines 1 1 *txt*)
+(strlines 1 2 *txt*)
+(strlines 1 3 *txt*)
+(strlines 1 100 *txt*)
+(strlines 2 2 *txt*)
+(strlines 2 3 *txt*)
+(strlines 2 100 *txt*)
+
+(strlines 2 4 *txt*)
+(strlines 2 5 *txt*)
+(strlines 2 6 *txt*)
+(strlines 2 7 *txt*)
+
+(strlines 7 7 *txt*)
+(strlines 7 4 *txt*)
+
+||#
