books/str/strrpos.lisp
@@ -1,0 +1,194 @@
+; ACL2 String Library
+; Copyright (C) 2009-2010 Centaur Technology
+;
+; Contact:
+;   Centaur Technology Formal Verification Group
+;   7600-C N. Capital of Texas Highway, Suite 300, Austin, TX 78731, USA.
+;   http://www.centtech.com/
+;
+; This program is free software; you can redistribute it and/or modify it under
+; the terms of the GNU General Public License as published by the Free Software
+; Foundation; either version 2 of the License, or (at your option) any later
+; version.  This program is distributed in the hope that it will be useful but
+; WITHOUT ANY WARRANTY; without even the implied warranty of MERCHANTABILITY or
+; FITNESS FOR A PARTICULAR PURPOSE.  See the GNU General Public License for
+; more details.  You should have received a copy of the GNU General Public
+; License along with this program; if not, write to the Free Software
+; Foundation, Inc., 51 Franklin Street, Suite 500, Boston, MA 02110-1335, USA.
+;
+; Original author: Jared Davis <jared@centtech.com>
+
+(in-package "STR")
+(include-book "strprefixp")
+(local (include-book "arithmetic"))
+
+(defund strrpos-fast (x y n xl yl)
+  (declare (type string x)
+           (type string y)
+           (type integer n)
+           (type integer xl)
+           (type integer yl)
+           (xargs :guard (and (stringp x)
+                              (stringp y)
+                              (natp xl)
+                              (natp yl)
+                              (natp n)
+                              (<= n (length y))
+                              (= xl (length x))
+                              (= yl (length y)))
+                  :measure (nfix n)))
+  ;; N goes from YL to 0.
+  (cond ((mbe :logic (prefixp (coerce x 'list)
+                              (nthcdr n (coerce y 'list)))
+              :exec (strprefixp-impl (the string x)
+                                     (the string y)
+                                     (the integer 0)
+                                     (the integer n)
+                                     (the integer xl)
+                                     (the integer yl)))
+         (mbe :logic (nfix n)
+              :exec n))
+        ((mbe :logic (zp n)
+              :exec (= (the integer n) (the integer 0)))
+         nil)
+        (t
+         (strrpos-fast (the string x)
+                       (the string y)
+                       (mbe :logic (- (nfix n) 1)
+                            :exec (the integer (- (the integer n) 1)))
+                       (the integer xl)
+                       (the integer yl)))))
+
+(defthm strpos-fast-type
+  (or (and (integerp (strrpos-fast x y n xl yl))
+           (<= 0 (strrpos-fast x y n xl yl)))
+      (not (strrpos-fast x y n xl yl)))
+  :rule-classes :type-prescription)
+
+(defthm strpos-fast-upper-bound
+  (implies (force (natp n))
+           (<= (strrpos-fast x y n xl yl) n))
+  :rule-classes :linear
+  :hints(("Goal" :in-theory (enable strrpos-fast))))
+
+(defthm strrpos-fast-when-empty
+  (implies (and (not (consp (coerce x 'list)))
+                (equal xl (length x))
+                (equal yl (length y))
+                (natp n))
+           (equal (STRRPOS-FAST X Y n xl yl)
+                  n))
+  :hints(("Goal" :in-theory (enable strrpos-fast))))
+
+
+
+(defund strrpos (x y)
+
+  ":Doc-Section Str
+  Locate the last occurrence of a substring~/
+
+  ~c[(strrpos x y)] searches through the string y for the last occurrence of the
+  substring x.  It returns NIL if x never occurs in y, or returns the index of
+  the first character of the last occurrence.
+
+  The function is \"efficient\" in the sense that it does not coerce its arguments
+  into lists, but rather traverses both strings with ~c[char].  On the other hand,
+  it is a naive string search which operates by repeatedly calling ~il[strprefixp],
+  rather than some better algorithm.
+
+  The \"soundness\" and \"completness\" of strpos are established in the theorems
+  ~c[prefixp-of-strrpos] and ~c[completeness-of-strrpos].~/~/"
+
+  (declare (type string x)
+           (type string y))
+  (let ((yl (length (the string y))))
+    (declare (type integer yl))
+    (strrpos-fast (the string x)
+                  (the string y)
+                  yl
+                  (the integer (length (the string x)))
+                  yl)))
+
+(defthm strrpos-type
+  (or (and (integerp (strrpos x y))
+           (<= 0 (strrpos x y)))
+      (not (strrpos x y)))
+  :rule-classes :type-prescription)
+
+
+
+(encapsulate
+ ()
+ (local (defthm lemma
+          (implies (and (stringp x)
+                        (stringp y)
+                        (natp xl)
+                        (natp yl)
+                        (natp n)
+                        (<= n (length y))
+                        (= xl (length x))
+                        (= yl (length y))
+                        (strrpos-fast x y n xl yl))
+                   (prefixp (coerce x 'list)
+                            (nthcdr (strrpos-fast x y n xl yl)
+                                    (coerce y 'list))))
+          :hints(("Goal"
+                  :in-theory (enable strrpos-fast)
+                  :induct (strrpos-fast x y n xl yl)))))
+
+ (defthm prefixp-of-strrpos
+   (implies (and (strrpos x y)
+                 (force (stringp x))
+                 (force (stringp y)))
+            (prefixp (coerce x 'list)
+                     (nthcdr (strrpos x y) (coerce y 'list))))
+   :hints(("Goal" :in-theory (enable strrpos)))))
+
+
+(encapsulate
+ ()
+ (local (defun my-induction (x y n m xl yl)
+          (declare (xargs :measure (nfix n)))
+          (cond ((prefixp (coerce x 'list)
+                          (nthcdr n (coerce y 'list)))
+                 nil)
+                ((zp n)
+                 (list x y n m xl yl))
+                (t
+                 (my-induction x y
+                               (- (nfix n) 1)
+                               (if (= (nfix n) (nfix m))
+                                   (- (nfix m) 1)
+                                 m)
+                               xl yl)))))
+
+ (local (defthm lemma
+          (implies (and (stringp x)
+                        (stringp y)
+                        (natp xl)
+                        (natp yl)
+                        (natp n)
+                        (natp m)
+                        (>= n m)
+                        (<= n (length y))
+                        (= xl (length x))
+                        (= yl (length y))
+                        (prefixp (coerce x 'list)
+                                 (nthcdr m (coerce y 'list))))
+                   (and (natp (strrpos-fast x y n xl yl))
+                        (>= (strrpos-fast x y n xl yl) m)))
+          :hints(("Goal"
+                  :in-theory (enable strrpos-fast)
+                  :induct (my-induction x y n m xl yl)
+                  :do-not '(generalize fertilize)))))
+
+ (defthm completeness-of-strrpos
+   (implies (and (prefixp (coerce x 'list)
+                          (nthcdr m (coerce y 'list)))
+                 (< m (len y))
+                 (force (natp m))
+                 (force (stringp x))
+                 (force (stringp y)))
+            (and (natp (strrpos x y))
+                 (>= (strrpos x y) m)))
+   :hints(("Goal" :in-theory (enable strrpos)))))
