books/tools/include-raw.lisp
@@ -1,0 +1,160 @@
+; Include raw Lisp files in ACL2 books
+; Copyright (C) 2010 Centaur Technology
+;
+; Contact:
+;   Centaur Technology Formal Verification Group
+;   7600-C N. Capital of Texas Highway, Suite 300, Austin, TX 78731, USA.
+;   http://www.centtech.com/
+;
+; This program is free software; you can redistribute it and/or modify it under
+; the terms of the GNU General Public License as published by the Free Software
+; Foundation; either version 2 of the License, or (at your option) any later
+; version.  This program is distributed in the hope that it will be useful but
+; WITHOUT ANY WARRANTY; without even the implied warranty of MERCHANTABILITY or
+; FITNESS FOR A PARTICULAR PURPOSE.  See the GNU General Public License for
+; more details.  You should have received a copy of the GNU General Public
+; License along with this program; if not, write to the Free Software
+; Foundation, Inc., 51 Franklin Street, Suite 500, Boston, MA 02110-1335, USA.
+;
+; Original authors: Jared Davis and Sol Swords <{jared,sswords}@centtech.com>
+
+
+(in-package "ACL2")
+
+(defttag include-raw)
+
+(progn!
+ (set-raw-mode t)
+
+ (defun raw-compile (name error-on-fail on-fail state)
+   (handler-case
+    (compile-file (extend-pathname (cbd) name state))
+    (error (condition)
+           (if error-on-fail
+               (let ((condition-str (format nil "~a" condition)))
+                 (er hard 'include-raw
+                     "Compilation of ~x0 failed with the following message:~%~@1~%"
+                     name condition-str))
+             (eval `(let ((condition ',condition))
+                      (declare (ignorable condition))
+                      ,on-fail)))))
+   nil)
+
+ (defun raw-load-uncompiled (name error-on-fail on-fail state)
+   (handler-case
+    (load (extend-pathname (cbd) name state))
+    (error (condition)
+           (if error-on-fail
+               (let ((condition-str (format nil "~a" condition)))
+                 (er hard 'include-raw
+                     "Load of ~x0 failed with the following message:~%~@1~%"
+                     name condition-str))
+             (eval `(let ((condition ',condition))
+                      (declare (ignorable condition))
+                      ,on-fail)))))
+   nil)
+
+ (defun raw-load (name error-on-fail on-fail state)
+   (let* ((fname (extend-pathname (cbd) name state))
+          (compiled-fname (compile-file-pathname fname)))
+     (handler-case
+      (load compiled-fname)
+      (error (condition)
+             (format t "Compiled file ~a failed to load; loading uncompiled ~a.~%Message: ~a~%"
+                     (namestring compiled-fname)
+                     fname condition)
+             (raw-load-uncompiled name error-on-fail on-fail state))))
+   nil))
+
+
+(defmacro include-raw (fname &key
+                             (do-not-compile 'nil)
+                             (on-compile-fail 'nil on-compile-fail-p)
+                             (on-load-fail 'nil on-load-fail-p))
+  ":doc-section miscellaneous
+Include a raw Lisp file in an ACL2 book, with compilation~/
+
+Note:  You must have a TTAG defined in order to use this macro.
+
+Usage:
+~bv[]
+ (include-raw \"my-raw-lisp-file.lsp\")
+ (include-raw \"a-raw-lisp-file.lsp\"
+              :on-compile-fail
+              (format t \"Compilation failed with message ~a~%\"
+                      condition)
+              :on-load-fail
+              (cw \"Oh well, the load failed~%\"))
+ (include-raw \"another-raw-lisp-file.lsp\"
+              :do-not-compile t)
+~ev[]
+
+The path of the raw Lisp file must be given relative to the book containing the
+include-raw form.
+
+By default, the raw Lisp file will be compiled and loaded when the containing
+book is certified.  When including the book, the compiled file will be loaded
+if possible, otherwise the original file will be loaded instead.  By default,
+if either compilation or loading fails, an error will occur.
+
+The optional keywords ~c[:on-compile-fail] and/or ~c[:on-load-fail] may be used
+to suppress the error for failed compilation or loading, respectively; their
+argument is a term which will be evaluated in lieu of producing an error.  When
+evaluating this term, the variable ~c[CONDITION] is bound to a value describing
+the failure; see Common Lisp documentation on ~c[HANDLER-CASE].
+
+The optional keyword ~c[:do-not-compile] may be used to suppress compilation.
+In this case, during book certification the file will just be loaded using
+~c[load].  Similarly, during include-book we will only load the lisp file, and
+not try to load a compiled file.
+
+One further note:  In most or all Lisps, compiling foo.lisp and foo.lsp results
+in the same compiled file (named foo.fasl, or something similar depending on
+the Lisp.)  Therefore, it is a mistake to use the same base name for a raw Lisp
+file with .lsp extension and an ACL2 book with .lisp extension, at least when
+using this tool and depending on compilation.~/~/"
+  `(progn
+     (make-event
+      (mv-let (erp val state)
+        ;; This progn!, including the compilation of the file to be loaded,
+        ;; will only happen during make-event expansion; that is, during
+        ;; certification, top-level evaluation, or uncertified inclusion (any
+        ;; other situations?)  Is this correct behavior?
+        ;;  - It is intentional that this _does_ happen during
+        ;; certification, which seems like a good time to compile files
+        ;; associated with the book being certified; in particular, hopefully
+        ;; the same book is not being certified multiple times simultaneously.
+        ;;  - It is intentional that this does _not_ happen during
+        ;; certified inclusion, because this may interfere with parallel
+        ;; certification: certifications of several files may simultaneously
+        ;; include the containing book and try to compile the file, stomping
+        ;; over each other's output.  Furthermore, if the book is certified,
+        ;; then the compiled file should already exist.
+        ;;  - In top-level evaluation/uncertified inclusion, it seems like a
+        ;; toss-up.  We prefer to perform the compilation to ensure the
+        ;; compiled file exists, so that compiled code is loaded and
+        ;; subsequent performance (in Lisps that don't compile automatically)
+        ;; is similar to that obtained by loading the certified book.  On the
+        ;; other hand, it might be argued that include-book should never cause
+        ;; a file to be written, on the grounds that it's likely an unexpected
+        ;; side-effect.  Perhaps in the future we might allow the user to
+        ;; customize what happens in each of these situations.
+        (progn!
+         (set-raw-mode t)
+         (unless ,do-not-compile
+           (raw-compile ,fname ,(not on-compile-fail-p)
+                        ',on-compile-fail state)))
+        (declare (ignore erp val))
+        (value '(value-triple :invisible))))
+
+     (progn!
+      (set-raw-mode t)
+      ;; According to Matt K., *hcomp-fn-restore-ht* is nonnil only when
+      ;; loading a book's compiled file.  We want to wait until the events of
+      ;; the include-book are being processed to run this, so that our compiled
+      ;; file isn't loaded twice.
+      (when (null *hcomp-fn-restore-ht*)
+        (,(if do-not-compile 'raw-load-uncompiled 'raw-load)
+         ,fname ,(not on-load-fail-p) ',on-load-fail state))
+      (value-triple ,fname))))
+
